concurrency/Modular/bst_inst.v
@@ -1,7 +1,6 @@
 Require Import VST.concurrency.conclib.
 Require Import VST.floyd.proofauto.
 Require Import VST.atomics.general_locks.
-Require Import Coq.Sets.Ensembles.
 Require Import bst.puretree.
 Require Import bst.bst.
 Require Import bst.dataStruct.
@@ -102,4 +101,89 @@ Proof.
     entailer !.
 Qed.
 
+Check enums.
+Check tint.
+
+Definition surely_malloc_spec :=
+  DECLARE _surely_malloc
+   WITH t: type, gv: globals
+   PRE [ size_t ]
+       PROP (and (Z.le 0 (sizeof t)) (Z.lt (sizeof t) Int.max_unsigned);
+                complete_legal_cosu_type t = true;
+                natural_aligned natural_alignment t = true)
+       PARAMS (Vptrofs (Ptrofs.repr (sizeof t))) GLOBALS (gv)
+       SEP (mem_mgr gv)
+    POST [ tptr tvoid ]
+    EX p: _,
+       PROP ()
+       RETURN (p)
+       SEP (mem_mgr gv; malloc_token Ews t p * data_at_ Ews t p).
+
+Check enums.
+
+Definition insertOp_spec :=
+  DECLARE _insertOp
+    WITH b: val, sh: share, x: Z, stt: Z,  v: val, p: val, tp: val, min: Z, max: Z, gv: globals
+  PRE [ tptr tvoid, tint, tptr tvoid, tint ]
+  PROP (writable_share sh; repable_signed min; repable_signed max; repable_signed x;
+        is_pointer_or_null v )
+  PARAMS (p; Vint (Int.repr x); v; Vint (Int.repr stt))
+  GLOBALS (gv)
+  SEP (mem_mgr gv;
+       (* data_at sh (t_struct_pn) (p, p) b; *)
+       field_at Ews t_struct_tree_t (DOT _t) tp p;
+       field_at Ews t_struct_tree_t (DOT _min) (Vint (Int.repr min)) p;
+       field_at Ews t_struct_tree_t (DOT _max) (Vint (Int.repr max)) p )
+  POST[ tvoid ]
+  EX (pnt p1' p2' : val) (lock1 lock2 : val),
+  PROP (pnt <> nullval)
+  LOCAL ()
+  SEP (mem_mgr gv;
+       (* data_at sh t_struct_pn (p, p) b; *)
+       field_at Ews t_struct_tree_t (DOT _t) pnt p;
+       malloc_token Ews t_struct_tree pnt;
+       malloc_token Ews t_struct_tree_t p1'; malloc_token Ews t_struct_tree_t p2';
+       atomic_int_at Ews (vint 0) lock1; atomic_int_at Ews (vint 0) lock2;
+       data_at Ews t_struct_tree (vint x, (v, (p1', p2'))) pnt;
+       data_at Ews t_struct_tree_t (Vlong (Int64.repr 0), (lock2, (vint x, vint max))) p2';
+       data_at Ews t_struct_tree_t (Vlong (Int64.repr 0), (lock1, (vint min, vint x))) p1';
+       field_at Ews t_struct_tree_t (DOT _min) (vint min) p;
+       field_at Ews t_struct_tree_t (DOT _max) (vint max) p).
+
+Definition Gprog : funspecs :=
+    ltac:(with_library prog [acquire_spec; release_spec; makelock_spec;
+     surely_malloc_spec; insertOp_spec (* ; traverse_spec; insert_spec; treebox_new_spec*) ]).
+(* Proving insertOp satisfies spec *)
+Lemma insertOp: semax_body Vprog Gprog f_insertOp insertOp_spec.
+Proof.
+  start_function.
+  forward.
+  forward_call (t_struct_tree_t, gv).
+  Intros p1.
+  forward_call (t_struct_tree_t, gv).
+  Intros p2.
+  forward.
+  assert_PROP (field_compatible t_struct_tree_t [] p1) by entailer!.
+  assert_PROP (field_compatible t_struct_tree_t [] p2) by entailer!.
+  forward. 
+  forward_call (gv).
+  Intros lock1.
+  forward.
+  sep_apply atomic_int_isptr.
+  Intros.
+  forward_call release_nonatomic (lock1).
+  forward_call (gv).
+  Intros lock2.
+  forward.
+  Intros.
+  forward_call release_nonatomic (lock2).
+  (* make lock invariant *)
+  forward_call (t_struct_tree, gv).
+  Intros pnt.
+  forward. forward. forward. forward. forward. forward. forward.
+  forward. forward. forward. forward. forward. forward. forward.
+  forward. 
+  Exists pnt p1 p2 lock1 lock2.
+  entailer !.
+Qed.
 
